theories_eval/LevelTwo_mut.v
@@ -1,0 +1,619 @@
+From Prototype Require Import Prelude Sig LevelOne.
+
+Module Make (S : Sig).
+Module O := LevelOne.Make (S).
+Definition arg_ty := @arg_ty (base S.t).
+
+(*********************************************************************************)
+(** *** Quoted naturals and explicit renamings. *)
+(*********************************************************************************)
+
+(** Quoted natural. *)
+Inductive qnat :=
+| Q_zero : qnat 
+| Q_succ : qnat -> qnat 
+| Q_mvar : nat -> qnat.
+
+Notation "'Q_one'" := (Q_succ Q_zero).
+
+(** Explicit renaming. *)
+Inductive ren :=
+| R_shift : qnat -> ren
+| R_cons : qnat -> ren -> ren
+| R_comp : ren -> ren -> ren 
+| R_mvar : O.ren -> ren.
+
+(*********************************************************************************)
+(** *** Expressions and explicit substitutions. *)
+(*********************************************************************************)
+
+(** Kind of an expression. *)
+Inductive kind :=
+(** Term. *)
+| Kt : kind
+(** Constructor argument. *)
+| Ka : arg_ty -> kind
+(** List of constructor arguments. *)
+| Kal : list arg_ty -> kind.
+Derive NoConfusion for kind.
+
+Definition eval_kind (k : kind) : O.kind :=
+  match k with Kt => O.Kt | Ka ty => O.Ka ty | Kal tys => O.Kal tys end.
+
+(** Type of an expressions metavariable. *)
+Definition mvar (k : kind) := O.expr (eval_kind k).
+
+(** Notations for expressions with known kinds. *)
+Reserved Notation "'term'" (at level 0).
+Reserved Notation "'arg' ty" (at level 0, ty at level 0).
+Reserved Notation "'args' tys" (at level 0, tys at level 0).
+
+(** Expressions over an abstract signature. 
+    Expressions are indexed by a kind: this is to avoid having too many 
+    distinct constructors for instantiation. *)
+Inductive expr : kind -> Type :=
+
+(** Variable term constructor (de Bruijn index). *)
+| E_tvar : qnat -> term
+(** Non-variable term constructor, applied to a list of arguments. *)
+| E_tctor : forall c, args (ctor_type S.t c) -> term
+
+(** Empty argument list. *)
+| E_al_nil : args []
+(** Non-empty argument list. *)
+| E_al_cons {ty tys} : arg ty -> args tys -> args (ty :: tys)
+
+(** Base argument (e.g. bool or string). *)
+| E_abase : forall b, denote_base S.t b -> arg (AT_base b)
+(** Term argument. *)
+| E_aterm : term -> arg AT_term
+(** Binder argument. *)
+| E_abind {ty} : arg ty -> arg (AT_bind ty)
+
+(** Instantiate an expressions with a renaming. *)
+| E_ren {k} : expr k -> ren -> expr k
+(** Instantiate an expressions with a substitution. *)
+| E_subst {k} : expr k -> subst -> expr k
+(** Expression metavariable. *)
+| E_mvar {k} : mvar k -> expr k
+
+with subst :=
+(** Shift substitution. *)
+| S_shift : qnat -> subst
+(** Substitution expansion. *)
+| S_cons : term -> subst -> subst
+(** Substitution composition. *)
+| S_comp : subst -> subst -> subst
+(** View a renaming as a substitution. *)
+| S_ren : ren -> subst
+(** Substitution metavariable. *)
+| S_mvar : O.subst -> subst
+
+where "'term'" := (expr Kt)
+  and "'arg' ty" := (expr (Ka ty))
+  and "'args' tys" := (expr (Kal tys)).
+
+(** Notations for common expressions. *)
+
+(*Notation "'↑ᵣ' k" := (R_shift k) (at level 0, k at level 0).
+Notation "i '.ᵣ' r" := (R_cons i r) (at level 60, right associativity).
+Notation "r1 '>>ᵣ' r2" := (R_comp r1 r2) (at level 50, left associativity).
+
+Notation "'↑ₛ' k" := (E_sshift k) (at level 0, k at level 0).
+Notation "t '.ₛ' s" := (E_scons t s) (at level 60, right associativity).
+Notation "s1 '>>ₛ' s2" := (E_scomp s1 s2) (at level 50, left associativity).
+
+Notation "t '[ᵣ' s ']'" := (E_rinst t s) (at level 15, s at level 0, no associativity).
+Notation "t '[ₛ' s ']'" := (E_sinst t s) (at level 15, s at level 0, no associativity).*)
+
+(** The identity renaming. *)
+Notation "'rid'" := (R_shift Q_zero).
+
+(** The identity substitution. *)
+Notation "'sid'" := (S_shift Q_zero).
+
+(** Lift a renaming through a binder. *)
+Definition up_ren (r : ren) : ren :=
+  R_cons Q_zero (R_comp r (R_shift Q_one)).
+
+(** Lift a substitution through a binder. *)
+Definition up_subst (s : subst) : subst :=
+  S_cons (E_tvar Q_zero) (S_comp s (S_shift Q_one)).
+
+(*********************************************************************************)
+(** *** Evalutation. *)
+(*********************************************************************************)
+
+Equations eval_qnat : qnat -> nat :=
+eval_qnat Q_zero := 0 ;
+eval_qnat (Q_succ i) := S (eval_qnat i) ;
+eval_qnat (Q_mvar x) := x.
+
+Equations eval_ren : ren -> O.ren :=
+eval_ren (R_shift i) := O.rshift (eval_qnat i) ;
+eval_ren (R_cons i r) := O.rcons (eval_qnat i) (eval_ren r) ;
+eval_ren (R_comp r1 r2) := O.rcomp (eval_ren r1) (eval_ren r2) ;
+eval_ren (R_mvar x) := x.
+
+Equations eval_expr {k} : expr k -> O.expr (eval_kind k) :=
+eval_expr (E_tvar i) := O.E_var (eval_qnat i) ;
+eval_expr (E_tctor c al) := O.E_ctor c (eval_expr al) ;
+eval_expr E_al_nil := O.E_al_nil ;
+eval_expr (E_al_cons a al) := O.E_al_cons (eval_expr a) (eval_expr al) ;
+eval_expr (E_abase b x) := O.E_abase b x ;
+eval_expr (E_aterm t) := O.E_aterm (eval_expr t) ;
+eval_expr (E_abind a) := O.E_abind (eval_expr a) ;
+eval_expr (E_ren e r) := O.rename (eval_expr e) (eval_ren r) ;
+eval_expr (E_subst e s) := O.substitute (eval_expr e) (eval_subst s) ;
+eval_expr (E_mvar x) := x
+
+with eval_subst : subst -> O.subst :=
+eval_subst (S_shift k) := O.sshift (eval_qnat k) ;
+eval_subst (S_cons t s) := O.scons (eval_expr t) (eval_subst s) ;
+eval_subst (S_comp s1 s2) := O.scomp (eval_subst s1) (eval_subst s2) ;
+eval_subst (S_ren r) := O.rscomp (eval_ren r) O.E_var ;
+eval_subst (S_mvar x) := x.
+
+(*********************************************************************************)
+(** *** Reification. *)
+(*********************************************************************************)
+
+(** Add a natural with a quoted natural. *)
+Equations qadd_aux : nat -> qnat -> qnat :=
+qadd_aux x Q_zero := Q_mvar x ;
+qadd_aux x (Q_succ y) := Q_succ (qadd_aux x y) ;
+qadd_aux x (Q_mvar y) := Q_mvar (x + y).    
+
+Lemma qadd_aux_sound x y : eval_qnat (qadd_aux x y) = x + eval_qnat y.
+Proof. funelim (qadd_aux x y) ; simp eval_qnat ; lia. Qed.
+#[global] Hint Rewrite qadd_aux_sound : eval_qnat.
+
+(** Add two quoted naturals. *)
+Equations qadd : qnat -> qnat -> qnat :=
+qadd Q_zero y := y ;
+qadd (Q_succ x) y := Q_succ (qadd x y) ;
+qadd (Q_mvar x) y := qadd_aux x y.
+
+Lemma qadd_sound x y : 
+  eval_qnat (qadd x y) = eval_qnat x + eval_qnat y.
+Proof. funelim (qadd x y) ; simp eval_qnat ; lia. Qed.
+#[global] Hint Rewrite qadd_sound : eval_qnat.
+
+Ltac2 rec reify_nat (t : constr) : constr := 
+  lazy_match! t with 
+  | 0 => constr:(Q_zero)
+  | S ?i =>
+    let i := reify_nat i in 
+    constr:(Q_succ $i)
+  | ?x + ?y => 
+    let x := reify_nat x in 
+    let y := reify_nat y in 
+    constr:(qadd $x $y)
+  | ?i => constr:(Q_mvar $i)
+  end
+
+with reify_ren (t : constr) : constr :=
+  lazy_match! t with 
+  | O.rshift ?k =>
+    let k := reify_nat k in 
+    constr:(R_shift $k) 
+  | O.rcons ?i ?r =>
+    let i := reify_nat i in 
+    let r := reify_ren r in 
+    constr:(R_cons $i $r)
+  | O.rcomp ?r1 ?r2 =>
+    let r1 := reify_ren r1 in 
+    let r2 := reify_ren r2 in 
+    constr:(R_comp $r1 $r2)
+  | ?r => constr:(R_mvar $r)
+  end.
+
+Ltac2 rec reify_expr (t : constr) : constr :=
+  lazy_match! t with 
+  | O.E_var ?i => 
+    let i := reify_nat i in
+    constr:(E_tvar $i)
+  | O.E_ctor ?c ?al => 
+    let al := reify_expr al in
+    constr:(E_tctor $c $al)
+  | O.E_al_nil => constr:(E_al_nil)
+  | O.E_al_cons ?a ?al => 
+    let a := reify_expr a in
+    let al := reify_expr al in
+    constr:(E_al_cons $a $al)
+  | O.E_abase ?b ?x => constr:(E_abase $b $x)
+  | O.E_aterm ?t => 
+    let t := reify_expr t in
+    constr:(E_aterm $t)
+  | O.E_abind ?a =>
+    let a := reify_expr a in
+    constr:(E_abind $a)
+  | O.rename ?t ?r =>
+    let t := reify_expr t in
+    let r := reify_ren r in
+    constr:(E_ren $t $r)
+  | O.substitute ?t ?s =>
+    let t := reify_expr t in
+    let s := reify_subst s in
+    constr:(E_subst $t $s)
+  | _ => constr:(@E_mvar Kt $t)
+  end
+
+with reify_subst (s : constr) : constr :=
+  lazy_match! s with 
+  | O.sid => constr:(sid)
+  | O.sshift ?k => 
+    let k := reify_nat k in 
+    constr:(S_shift $k)
+  | O.scons ?t ?s =>
+    let t := reify_expr t in 
+    let s := reify_subst s in 
+    constr:(S_cons $t $s)
+  | O.scomp ?s1 ?s2 =>
+    let s1 := reify_subst s1 in 
+    let s2 := reify_subst s2 in 
+    constr:(S_comp $s1 $s2)
+  | O.srcomp ?s ?r =>
+    let s := reify_subst s in 
+    let r := reify_ren r in
+    constr:(S_comp $s (S_ren $r))
+  | O.rscomp ?r ?s =>
+    let r := reify_ren r in
+    let s := reify_subst s in 
+    constr:(S_comp (S_ren $r) $s)
+  | ?s => constr:(S_mvar $s)
+  end.
+  
+(*********************************************************************************)
+(** *** Normal forms. *)
+(*********************************************************************************)
+
+(** The goal of normal forms is not to precisely capture the structure
+    of simplified terms/substitutions: rather, they add some structure 
+    above plain terms/substitutions, while still remaining simple to work with.
+    
+    In particular, normal forms are not unique, and all functions 
+    [term -> nf_term] are not equivalent. *)
+
+(** Normal form renamings: the left hand side of a composition
+    can't be a cons or a composition. *)
+Inductive nf_ren : Type :=
+(** [NR_shift k] represents [R_shift k]. *)
+| NR_shift : qnat -> nf_ren
+(** [NR_cons i r] represents [R_cons i r]. *)
+| NR_cons : qnat -> nf_ren -> nf_ren 
+(** [NR_comp_shift k r] represents [R_comp (R_shift k) r]. *)
+| NR_comp_shift : qnat -> nf_ren -> nf_ren 
+(** [NR_comp_mvar x r] represents [R_comp (R_mvar x) r]. *)
+| NR_comp_mvar : O.ren -> nf_ren -> nf_ren 
+(** [NR_mvar x] represents [R_mvar x]. *)
+| NR_mvar : O.ren -> nf_ren.
+
+Reserved Notation "'nf_term'" (at level 0).
+Reserved Notation "'nf_arg' ty" (at level 0, ty at level 0).
+Reserved Notation "'nf_args' tys" (at level 0, tys at level 0).
+
+Inductive nf_expr : kind -> Type :=
+| NE_tvar : qnat -> nf_term
+| NE_tctor : forall c, nf_args (ctor_type S.t c) -> nf_term
+| NE_al_nil : nf_args []
+| NE_al_cons {ty tys} : nf_arg ty -> nf_args tys -> nf_args (ty :: tys)
+| NE_abase : forall b, denote_base S.t b -> nf_arg (AT_base b)
+| NE_aterm : nf_term -> nf_arg AT_term
+| NE_abind {ty} : nf_arg ty -> nf_arg (AT_bind ty)
+| NE_mvar {k} : mvar k -> nf_expr k
+(** Renaming/substitution blocked on a metavariable. *)
+| NE_ren_mvar_r {k} : mvar k -> nf_ren -> nf_expr k
+| NE_subst_mvar_s {k} : mvar k -> nf_subst -> nf_expr k
+(** Renaming/susbtitution blocked on a variable. *)
+| NE_ren_var : qnat -> nf_ren -> nf_term
+| NE_subst_var : qnat -> nf_subst -> nf_term
+
+(** Normal form substitutions: the left hand side of a composition
+    can't be a cons or a composition. *)
+with nf_subst : Type :=
+| NS_shift : qnat -> nf_subst 
+| NS_cons : nf_term -> nf_subst -> nf_subst 
+| NS_comp_shift : qnat -> nf_subst -> nf_subst 
+| NS_comp_ren : nf_ren -> nf_subst -> nf_subst 
+| NS_comp_mvar : O.subst -> nf_subst -> nf_subst 
+| NS_ren : nf_ren -> nf_subst
+| NS_mvar : O.subst -> nf_subst
+
+where "'nf_term'" := (nf_expr Kt)
+  and "'nf_arg' ty" := (nf_expr (Ka ty))
+  and "'nf_args' tys" := (nf_expr (Kal tys)).
+
+Equations eval_nf_ren : nf_ren -> O.ren :=
+eval_nf_ren (NR_shift k) := O.rshift (eval_qnat k) ;
+eval_nf_ren (NR_cons i r) := O.rcons (eval_qnat i) (eval_nf_ren r) ;
+eval_nf_ren (NR_comp_shift k r) := O.rcomp (O.rshift (eval_qnat k)) (eval_nf_ren r) ;
+eval_nf_ren (NR_comp_mvar x r) := O.rcomp x (eval_nf_ren r) ;
+eval_nf_ren (NR_mvar x) := x.
+
+Equations eval_nf_expr {k} : nf_expr k -> O.expr (eval_kind k) :=
+eval_nf_expr (NE_tvar i) := O.E_var (eval_qnat i) ;
+eval_nf_expr (NE_tctor c al) := O.E_ctor c (eval_nf_expr al) ;
+eval_nf_expr NE_al_nil := O.E_al_nil ;
+eval_nf_expr (NE_al_cons a al) := O.E_al_cons (eval_nf_expr a) (eval_nf_expr al) ;
+eval_nf_expr (NE_abase b x) := O.E_abase b x ;
+eval_nf_expr (NE_aterm t) := O.E_aterm (eval_nf_expr t) ;
+eval_nf_expr (NE_abind a) := O.E_abind (eval_nf_expr a) ;
+eval_nf_expr (NE_mvar x) := x ;
+eval_nf_expr (NE_ren_mvar x r) := O.rename x (eval_nf_ren r) ;
+eval_nf_expr (NE_subst_mvar x s) := O.substitute x (eval_nf_subst s) ;
+eval_nf_expr (NE_ren_var i r) := eval_nf_ren r (eval_qnat i) ;
+eval_nf_expr (NE_subst_var i s) := eval_nf_subst s (eval_qnat i) 
+
+with eval_nf_subst : nf_subst -> O.subst :=
+eval_nf_subst (NS_shift k) := O.sshift k ;
+eval_nf_subst (NS_cons t s) := O.scons (eval_nf_expr t) (eval_nf_subst s) ;
+eval_nf_subst (NS_comp_shift k s) := O.scomp 
+.
+
+(*********************************************************************************)
+(** *** Simplification. *)
+(*********************************************************************************)
+
+
+(** Apply a normal form renaming to a quoted natural. *)
+Equations rapply : nf_ren -> qnat -> qnat :=
+rapply (NR_shift k) i := qadd k i ;
+rapply (NR_cons k _) Q_zero := k ;
+rapply (NR_cons _ r) (Q_succ i) := rapply r i ;
+rapply (NR_cons k r) (Q_mvar i) := Q_mvar (eval_nf_ren (NR_cons k r) i) ;
+rapply (NR_comp_shift k r) i := rapply r (qadd k i) ;
+rapply (NR_comp_mvar x r) i := rapply r (Q_mvar (x (eval_qnat i))) ;
+rapply (NR_mvar x) i := Q_mvar (x (eval_qnat i)).
+
+Lemma rapply_sound r i : 
+  eval_qnat (rapply r i) = eval_ren r (eval_qnat i).
+Proof. 
+funelim (rapply r i) ; simp eval_qnat eval_ren ; try solve [ auto ].
+rewrite H0, H. reflexivity.
+Qed.
+#[global] Hint Rewrite rapply_sound : eval_qnat.
+
+(** Tail of a normal form renaming. *)
+Equations rtail : nf_ren -> nf_ren := 
+rtail (N_rshift k) := N_rshift (qS k) ;
+rtail (N_rcons _ r) := r ;
+rtail (N_rcomp k xr r) := N_rcomp (qS k) xr r.
+
+Lemma rtail_sound r : eval_nf (rtail r) =₁ O.rcomp (O.rshift 1) (eval_nf r).
+Proof. 
+funelim (rtail r) ; simp rtail eval_nf eval_qnat.
+- now rewrite O.rshift_succ_l.
+- now rewrite O.rshift_rcons.
+- repeat rewrite <-O.rcomp_assoc. now rewrite O.rshift_succ_l.
+Qed. 
+#[global] Hint Rewrite rtail_sound : eval_nf.    
+
+(** Drop the first [k] elements in a normal form renaming. *)
+Equations rdrop : qnat -> nf_ren -> nf_ren :=
+rdrop q0 r := r ;
+rdrop (qS k) r := rtail (rdrop k r) ;
+rdrop (qAtom k) r := N_rcomp (qAtom k) O.rid r.
+
+Lemma rdrop_sound k r : 
+  eval_nf (rdrop k r) =₁ O.rcomp (O.rshift (eval_qnat k)) (eval_nf r).
+Proof.
+funelim (rdrop k r) ; simp eval_nf eval_qnat.
+- now rewrite O.rcomp_rid_l.
+- rewrite H. now rewrite <-O.rcomp_assoc, O.rshift_succ_l.
+- now rewrite O.rcomp_rid_r. 
+Qed.  
+#[global] Hint Rewrite rdrop_sound : eval_nf.    
+
+(** Apply a normal form renaming to a de Bruijn index. *)
+Equations rapply : nf_ren -> qnat -> qnat :=
+rapply (N_rshift k) i := qadd k i ;
+rapply (N_rcons i _) q0 := i ;
+rapply (N_rcons _ r) (qS k) := rapply r k ;
+rapply (N_rcons i r) (qAtom k) := qAtom (eval_nf (N_rcons i r) k) ;
+rapply (N_rcomp k xr r) i := rapply r (qAtom (xr (eval_qnat (qadd k i)))).
+
+Lemma rapply_sound r i : 
+  eval_qnat (rapply r i) = eval_nf r (eval_qnat i).
+Proof. funelim (rapply r i) ; now simp eval_nf eval_qnat in *. Qed.
+#[global] Hint Rewrite rapply_sound : eval_nf.    
+    
+(** Compose two normal form renamings. *)
+Equations rcomp : nf_ren -> nf_ren -> nf_ren :=
+rcomp (N_rshift k) r := rdrop k r ;
+rcomp (N_rcons i r1) r2 := N_rcons (rapply r2 i) (rcomp r1 r2) ;
+rcomp (N_rcomp k xr r1) r2 := N_rcomp k xr (rcomp r1 r2).
+
+Lemma rcomp_sound r1 r2 : 
+  eval_nf (rcomp r1 r2) =₁ O.rcomp (eval_nf r1) (eval_nf r2).
+Proof.
+funelim (rcomp r1 r2) ; simp eval_nf eval_qnat in *.
+- reflexivity.
+- now rewrite O.rcomp_rcons_distrib, H.
+- rewrite H. now repeat rewrite O.rcomp_assoc.
+Qed.
+#[global] Hint Rewrite rcomp_sound : eval_nf.    
+
+(** Lift a normal form renaming through a binder. *)
+Equations rup : nf_ren -> nf_ren :=
+rup r := N_rcons q0 (rcomp r (N_rshift q1)).
+
+Lemma rup_sound r : eval_nf (rup r) =₁ O.up_ren (eval_nf r).
+Proof. simp rup eval_nf. reflexivity. Qed.
+
+(** Instantiate a normal form term with a normal form renaming. *)
+Equations rinst {k} : nf_expr (K1 k) -> nf_ren -> nf_expr (K1 k) :=
+rinst (N_tvar i) r := N_tvar (rapply r i) ;
+rinst (N_tctor c al) r := N_tctor c (rinst al r) ;
+rinst N_al_nil _ := N_al_nil ;
+rinst (N_al_cons a al) r := N_al_cons (rinst a r) (rinst al r) ;
+rinst (N_abase b x) _ := N_abase b x ;
+rinst (N_aterm t) r := N_aterm (rinst t r) ;
+rinst (N_abind a) r := N_abind (rinst a (rup r)) ;
+rinst (N_rinst_l xt r1) r2 := N_rinst_l xt (rcomp r1 r2) ;
+rinst (N_sinst_l xt s) r := N_sinst_l xt (srcomp s r) ;
+rinst (N_rinst_r i xr r1) r2 := N_rinst_r i xr (rcomp r1 r2) ;
+rinst (N_sinst_r i xs s) r := N_sinst_r i xs (srcomp s r)
+
+(** Compose a normal form substitution with a normal form renaming. *)
+with srcomp : nf_subst -> nf_ren -> nf_subst :=
+srcomp (N_sshift k) r := N_sren (rdrop k r) ;
+srcomp (N_scons t s) r := N_scons (rinst t r) (srcomp s r) ;
+srcomp (N_scomp k xs s) r := N_scomp k xs (srcomp s r) ; 
+srcomp (N_sren r1) r2 := N_sren (rcomp r1 r2).
+
+Lemma rinst_srcomp_sound_aux : 
+  (forall k (t : nf_expr (K1 k)) r, 
+    eval_nf (rinst t r) = O.rename (eval_nf t) (eval_nf r)) *
+  (forall s r, 
+    eval_nf (srcomp s r) =₁ fun i => O.rename (eval_nf s i) (eval_nf r)).
+Proof.
+apply rinst_elim with 
+  (P := fun k (t : nf_expr (K1 k)) (r : nf_ren) (res : nf_expr (K1 k))  => 
+    eval_nf res = O.rename (eval_nf t) (eval_nf r))
+  (P0 := fun (s : nf_subst) (r : nf_ren) (res : nf_subst) =>
+    eval_nf res =₁ fun i => O.rename (eval_nf s i) (eval_nf r)).
+all: try (intros ; now simp eval_nf).
+- intros c al r H. simp eval_nf. rewrite H. now simp rename.
+- intros ty tys a al r H1 H2. simp eval_nf rename. now rewrite H1, H2.
+- intros t r H. simp eval_nf rename. now rewrite H.
+- intros ty a r H. simp eval_nf rename. now rewrite H, rup_sound.
+- intros k xt r1 r2. destruct k ; simp eval_nf ; now rewrite O.ren_ren.
+- intros k xt s r H. destruct k ; simp eval_nf ; now rewrite H, O.subst_ren.
+- intros i xs s r H. simp eval_nf substitute. cbv [O.scomp]. 
+  now rewrite H, O.subst_ren.
+- intros k r. simp eval_nf. intros i. rewrite rdrop_sound. reflexivity.
+- intros t s r H1 H2. simp eval_nf. rewrite H1, H2. intros [|i] ; reflexivity.
+- intros k xs s r H. simp eval_nf. rewrite H. intros i. cbv [O.scomp O.sshift].
+  simp substitute. now rewrite O.subst_ren.
+- intros r1 r2. simp eval_nf. intros i. simp rename. now rewrite rcomp_sound.
+Qed.
+
+Lemma rinst_sound k (t : nf_expr (K1 k)) r :   
+  eval_nf (rinst t r) = O.rename (eval_nf t) (eval_nf r).
+Proof. now apply rinst_srcomp_sound_aux. Qed.
+
+Lemma srcomp_sound s r :
+  eval_nf (srcomp s r) =₁ fun i => O.rename (eval_nf s i) (eval_nf r).
+Proof. now apply rinst_srcomp_sound_aux. Qed.
+
+(** Apply a normal form substitution to a de Bruijn index. *)
+Equations sapply : nf_subst -> qnat -> nf_term :=
+sapply (N_sshift k) i := N_tvar (qadd k i) ;
+sapply (N_scons t _) q0 := t ;
+sapply (N_scons _ s) (qS i) := sapply s i ;
+sapply (N_scons t s) (qAtom i) := @N_sinst_l Kt (eval_nf (N_scons t s) i) (N_sshift q0) ;
+sapply (N_scomp k xs s) i := N_sinst_r (qadd k i) xs s ;
+sapply (N_sren r) i := N_tvar (rapply r i).  
+
+Lemma sapply_sound s i : eval_nf (sapply s i) = eval_nf s i.
+Proof. 
+funelim (sapply s i) ; simp eval_nf ; try reflexivity.
+- now rewrite H.
+- now rewrite rapply_sound.
+Qed.    
+
+(** Tail of a normal form substitution. *)
+Equations stail : nf_subst -> nf_subst :=
+stail (N_sshift k) := N_sshift (S k) ;
+stail (N_scons t s) := s ;
+stail (N_scomp k xs s) := N_scomp (S k) xs s ;
+stail (N_sren r) := N_sren (rtail r).
+
+Lemma stail_sound s : eval_nf (stail s) =₁ O.scomp (O.sshift 1) (eval_nf s).
+Proof. 
+funelim (stail s) ; simp eval_nf.
+- now rewrite O.sshift_succ_l.
+- now rewrite O.sshift_scons.
+- repeat rewrite <-O.scomp_assoc. now rewrite O.sshift_succ_l.
+- intros i. now rewrite rtail_sound.
+Qed.
+
+(** Drop the first [k] elements in a normal form substitution. *)
+Equations sdrop : nat -> nf_subst -> nf_subst :=
+sdrop 0 s := s ;
+sdrop (S k) s := stail (sdrop k s).
+
+Lemma sdrop_sound k s : eval_nf (sdrop k s) =₁ O.scomp (O.sshift k) (eval_nf s).
+Proof.
+funelim (sdrop k s) ; simp eval_nf.
+- now rewrite O.scomp_sid_l.
+- rewrite stail_sound, H. now rewrite <-O.scomp_assoc, O.sshift_succ_l.
+Qed.  
+
+(** Lift a normal form substitution through a binder. *)
+Equations sup : nf_subst -> nf_subst :=
+sup s := N_scons (N_tvar 0) (srcomp s (N_rshift 1)).
+
+Lemma sup_sound s : eval_nf (sup s) =₁ O.up_subst (eval_nf s).
+Proof. simp sup eval_nf. unfold O.up_subst. now rewrite srcomp_sound. Qed.
+
+(** Compose a normal form renaming with a normal form substitution. *)
+Equations rscomp : nf_ren -> nf_subst -> nf_subst :=
+rscomp (N_rshift k) s := sdrop k s ;
+rscomp (N_rcons i r) s := N_scons (sapply s i) (rscomp r s) ;
+rscomp (N_rcomp k xr r) s := N_scomp k (fun i => O.E_var (xr i)) (rscomp r s).
+
+Lemma rscomp_sound r s : 
+  eval_nf (rscomp r s) =₁ fun i => eval_nf s (eval_nf r i).
+Proof.
+funelim (rscomp r s) ; simp eval_nf.
+- now rewrite sdrop_sound.
+- rewrite sapply_sound, H. intros [|] ; reflexivity.
+- now rewrite H.
+Qed.     
+
+(** Instantiate a normal form expression with a normal form substitution. *)
+Equations sinst {k} (t : nf_expr (K1 k)) (s : nf_subst) : nf_expr (K1 k) by struct t :=
+sinst (N_tvar i) s := sapply s i ;
+sinst (N_tctor c al) s := N_tctor c (sinst al s) ;
+sinst N_al_nil _ := N_al_nil ;
+sinst (N_al_cons a al) s := N_al_cons (sinst a s) (sinst al s) ;
+sinst (N_abase b x) _ := N_abase b x ;
+sinst (N_aterm t) s := N_aterm (sinst t s) ;
+sinst (N_abind a) s := N_abind (sinst a (sup s)) ;
+sinst (N_rinst_l xt r) s := N_sinst_l xt (rscomp r s) ;
+sinst (N_sinst_l xt s1) s2 := N_sinst_l xt (scomp s1 s2) ;
+sinst (N_rinst_r i xr r) s := N_sinst_r i (fun i => O.E_var (xr i)) (rscomp r s) ;
+sinst (N_sinst_r i xs s1) s2 := N_sinst_r i xs (scomp s1 s2)
+
+(** Compose two normal form substitutions. *)
+with scomp (s1 : nf_subst) (s2 : nf_subst) : nf_subst by struct s1 :=
+scomp (N_sshift k) s := sdrop k s ;
+scomp (N_scons t s1) s2 := N_scons (sinst t s2) (scomp s1 s2) ;
+scomp (N_scomp k xs s1) s2 := N_scomp k xs (scomp s1 s2) ; 
+scomp (N_sren r) s := rscomp r s.
+
+Lemma sinst_scomp_sound_aux : 
+  (forall k (t : nf_expr (K1 k)) s, 
+    eval_nf (sinst t s) = O.substitute (eval_nf t) (eval_nf s)) *
+  (forall s1 s2, 
+    eval_nf (scomp s1 s2) =₁ O.scomp (eval_nf s1) (eval_nf s2)).
+Proof.
+apply sinst_elim with 
+  (P := fun k (t : nf_expr (K1 k)) (s : nf_subst) (res : nf_expr (K1 k))  => 
+    eval_nf res = O.substitute (eval_nf t) (eval_nf s))
+  (P0 := fun (s1 s2 res : nf_subst) =>
+    eval_nf res =₁ O.scomp (eval_nf s1) (eval_nf s2)).
+- intros i s. now rewrite sapply_sound.
+- intros c al s H. simp eval_nf. now rewrite H.
+- reflexivity.
+- intros ty tys a al s H1 H2. simp eval_nf substitute. now rewrite H1, H2.
+- intros b x s. now simp eval_nf substitute.
+- intros t s H. simp eval_nf substitute. now rewrite H.
+- intros ty a s H. simp eval_nf substitute. now rewrite H, sup_sound.
+- intros k xt r s. destruct k ; simp eval_nf substitute.
+  all: now rewrite rscomp_sound, O.ren_subst.
+- intros k xt s1 s2 H. destruct k ; simp eval_nf substitute.
+  all: now rewrite H, O.subst_subst.
+- intros i xr r s. simp eval_nf substitute rename.
+  cbv [O.scomp]. simp substitute. now rewrite rscomp_sound.
+- intros i xs s1 s2 H. simp eval_nf substitute. 
+  cbv [O.scomp]. now rewrite H, O.subst_subst.
+- intros k s. simp eval_nf. now rewrite sdrop_sound.
+- intros t s1 s2 H1 H2. simp eval_nf. rewrite H1, H2.
+  now rewrite O.scomp_scons_distrib.
+- intros k xs s1 s2 H. simp eval_nf. rewrite H. now repeat rewrite O.scomp_assoc.
+- intros r s. rewrite rscomp_sound. reflexivity.
+Qed. 
+    
